\subsection{Altitude}

\[
m \ddot{z} = c_{\phi} c_{\theta} F_R - m g
\]

\[
\ddot{z} = \frac{c_{\phi} c_{\theta}}{m} F_R - g
\]

\[
e_3 = z_{ref} - z
\]

\[
\dot{e}_3 = \dot{z}_{ref} - \dot{z}
\]

\[
\dot{e}_3 = \dot{z}_{ref} - v_z
\]

\[
v_{z,ref} = c_3 e_3 + \dot{z}_{ref} + \lambda_3 \chi_3
\]

\[
e_4 = v_{z,ref} - v_z
\]

\[
\dot{e}_4 = \dot{v}_{z,ref} - \dot{v}_z
\]

\[
\dot{e}_4 = c_3 \dot{e}_3 + \ddot{z}_{ref} + \lambda_3 e_3 - \dot{v}_z
\]

\[
\dot{z}_{ref} = v_{z,ref} - c_3 e_3 - \lambda_3 \chi_3 
\]

\[
\dot{z}_{ref} = e_4 + v_z - c_3 e_3 - \lambda_3 \chi_3 
\]


\[
\dot{e}_3 = e_4 - c_3 e_3 - \lambda_3 \chi_3
\]

\[
\dot{e}_4 = c_3 \left( e_4 - c_3 e_3 - \lambda_3 \chi_3 \right) + \ddot{z}_{ref} + \lambda_3 e_3
- \left( \frac{c_{\phi} c_{\theta}}{m} F_R - g \right)
\]


\[
\dot{e}_4 = f_4(e_3,e_4)
\]

\[
F_R
= \frac{m}{c_{\phi} c_{\theta}} \left( -f_4(e_3,e_4)
+ c_3 \left( e_4 - c_3 e_3 - \lambda_3 \chi_3 \right) + \ddot{z}_{ref} + \lambda_3 e_3 + g \right)
\]










