\subsection{Position}

\[
\mathbf{e}_5 = \mathbf{x}_{ref} - \mathbf{x}
\]

\[
\dot{\mathbf{e}}_5 = \dot{\mathbf{x}}_{ref} - \dot{\mathbf{x}}
\]

\[
\dot{\mathbf{e}}_5 = \dot{\mathbf{x}}_{ref} - \mathbf{v}
\]

\[
\mathbf{v}_{ref} = \mathbf{C}_5 \mathbf{e}_5 + \dot{\mathbf{x}}_{ref} + \boldsymbol\Lambda_5 \boldsymbol\chi_5
\]

\[
\dot{\mathbf{v}}_{ref} = \mathbf{C}_5 \dot{\mathbf{e}}_5 + \ddot{\mathbf{x}}_{ref} + \boldsymbol\Lambda_5 \mathbf{e}_5
\]


\[
\mathbf{e}_6 = \mathbf{v}_{ref} - \mathbf{v}
\]

\[
\dot{\mathbf{e}}_6 = \dot{\mathbf{v}}_{ref} - \dot{\mathbf{v}}
\]

\[
\dot{\mathbf{e}}_6 = \mathbf{C}_5 \dot{\mathbf{e}}_5 + \ddot{\mathbf{x}}_{ref} + \boldsymbol\Lambda_5 \mathbf{e}_5 - \ddot{\mathbf{x}}
\]

\[
\dot{\mathbf{x}}_{ref} = \mathbf{v}_{ref} - \mathbf{C}_5 \mathbf{e}_5 - \boldsymbol\Lambda_5 \boldsymbol\chi_5
\]

\[
\dot{\mathbf{x}}_{ref} = \mathbf{e}_6 + \mathbf{v} - \mathbf{C}_5 \mathbf{e}_5 - \boldsymbol\Lambda_5 \boldsymbol\chi_5
\]

\[
\dot{\mathbf{e}}_5 = \mathbf{e}_6 - \mathbf{C}_5 \mathbf{e}_5 - \boldsymbol\Lambda_5 \boldsymbol\chi_5
\]

\[
\dot{\mathbf{e}}_6 = \mathbf{f}_6(\mathbf{e}_5,\mathbf{e}_6)
\]

\[
\mathbf{f}_6(\mathbf{e}_5,\mathbf{e}_6)
= \mathbf{C}_5 \left( \mathbf{e}_6 - \mathbf{C}_5 \mathbf{e}_5 - \boldsymbol\Lambda_5 \boldsymbol\chi_5 \right)
+ \ddot{\mathbf{x}}_{ref}
+ \boldsymbol\Lambda_5 \mathbf{e}_5
- \left(
\mathbf{g}
+ \frac{1}{m} \mathbf{F}_{R}
+ \frac{1}{m} \mathbf{F}_{D}
\right)
\]

\[
\mathbf{F}_{R}
= m \left(
-\mathbf{f}_6(\mathbf{e}_5,\mathbf{e}_6)
+ \mathbf{C}_5 \left( \mathbf{e}_6 - \mathbf{C}_5 \mathbf{e}_5 - \boldsymbol\Lambda_5 \boldsymbol\chi_5 \right)
+ \ddot{\mathbf{x}}_{ref}
+ \boldsymbol\Lambda_5 \mathbf{e}_5
- \mathbf{g}
- \frac{1}{m} \mathbf{F}_{D}
\right)
\]



