\subsection{Rotation}

\[
\mathbf{I} \dot{\boldsymbol\omega}
= \tau - \boldsymbol\omega \times \left( \mathbf{I} \boldsymbol\omega \right)
\]

\[
\dot{\boldsymbol\omega}
= \mathbf{I}^{-1} \left( \boldsymbol\tau - \boldsymbol\omega \times \left( \mathbf{I} \boldsymbol\omega \right) \right)
\]

\[
I =
\begin{bmatrix}
I_{xx} & 0 & 0 \\
0 & I_{yy} & 0 \\
0 & 0 & I_{zz}
\end{bmatrix}
\]

\subsubsection{Quaternion}


\[
\dot{\mathbf{q}} = \mathbf{A}_3 \boldsymbol\omega
\]

\[
\ddot{\mathbf{q}} = \dot{\mathbf{A}}_3 \boldsymbol\omega + \mathbf{A}_3 \dot{\boldsymbol\omega}
\]

\[
\ddot{\mathbf{q}}
= \dot{\mathbf{A}}_3 \boldsymbol\omega
+ \mathbf{A}_3 \mathbf{I}^{-1} \left( \boldsymbol\tau - \boldsymbol\omega \times \left( \mathbf{I} \boldsymbol\omega \right) \right)
\]

\subsubsection{Euler}

\[
\omega
=
\begin{bmatrix}
1 & 0		& -s_{\theta} \\
0 & c_{\phi}	& c_{\theta} s_{\phi} \\
0 & -s_{\phi}	& c_{\theta} s_{\phi}
\end{bmatrix}
\dot{\theta} 
= \mathbf{S} \dot{\theta}
\]

\[
\dot{\omega} = \dot{\mathbf{S}} \dot{\theta} + \mathbf{S} \ddot{\theta}
\]

\[
\ddot{\theta} =
\mathbf{S}^{-1} \left( \dot{\omega} - \dot{\mathbf{S}} \dot{\theta} \right)
\]

\begin{equation}
\ddot{\theta} =
\mathbf{S}^{-1} \left( I^{-1} \left( \tau - \omega \times \left( I \omega \right) \right) - \dot{\mathbf{S}} \dot{\theta} \right)
\label{eq:eom_theta}
\end{equation}



\[
\boldsymbol\tau_B =
\begin{bmatrix}
Lk \left( \gamma_1 - \gamma_3 \right) \\
Lk \left( \gamma_2 - \gamma_4 \right) \\
b \left( \gamma_1 - \gamma_2 + \gamma_3 - \gamma_4 \right)
\end{bmatrix}
=
\begin{bmatrix}
Lk & 0  & -Lk & 0 \\
0  & Lk & 0   & -Lk \\
b  & -b & b   & -b
\end{bmatrix}
\begin{bmatrix}
\gamma_1 \\ \gamma_2 \\ \gamma_3 \\ \gamma_4
\end{bmatrix}
\]






